Source/DafnyRuntime/DafnyRuntimeDafny/array.dfy
@@ -56,23 +56,41 @@ module {:options "/functionSyntax:4"} Arrays {
       requires Valid()
       requires i < Length()
       modifies Repr
+      ensures Valid()
+      ensures Repr == old(Repr)
       ensures values == old(values)[..i] + [Set(t)] + old(values)[(i + 1)..]
+      ensures Read(i) == t
 
-    method WriteRange(start: nat, from: Array<T>, fromStart: nat, fromEnd: nat)
+    method WriteRange(start: nat, from: seq<T>)
+      requires Valid()
+      requires start <= Length()
+      requires start + |from| <= Length()
+      modifies Repr
+      ensures Valid()
+      ensures Repr == old(Repr)
+      ensures values == 
+        old(values)[..start] + 
+        seq(|from|, i requires 0 <= i < |from| => Set(from[i])) + 
+        old(values)[(start + |from|)..]
+
+    method WriteRangeArray(start: nat, from: Array<T>, fromStart: nat, fromEnd: nat)
       requires Valid()
       requires from.Valid()
-      requires start < Length()
+      requires start <= Length()
       requires fromStart <= fromEnd <= from.Length()
       requires start + (fromEnd - fromStart) <= Length()
       requires forall i | fromStart <= i < fromEnd :: from.values[i].Set?
       requires Repr !! from.Repr
       modifies Repr
+      ensures Valid()
+      ensures Repr == old(Repr)
       ensures values == 
         old(values)[..start] + 
         from.values[fromStart..fromEnd] + 
         old(values)[(start + (fromEnd - fromStart))..]
   }
 
+  // Feasibility implementation
   class DafnyArray<T> extends Array<T> {
     var valuesArray: array<ArrayCell<T>>
 
@@ -98,6 +116,7 @@ module {:options "/functionSyntax:4"} Arrays {
     function Length(): nat
       requires Valid()
       reads Repr
+      ensures Length() == |values|
     {
       valuesArray.Length
     }
@@ -116,32 +135,56 @@ module {:options "/functionSyntax:4"} Arrays {
       requires Valid()
       requires i < Length()
       modifies Repr
+      ensures Valid()
+      ensures Repr == old(Repr)
+      ensures Length() == old(Length())
       ensures values == old(values)[..i] + [Set(t)] + old(values)[(i + 1)..]
+      ensures Read(i) == t
     {
       valuesArray[i] := Set(t);
 
       values := valuesArray[..];
     }
 
-    method WriteRange(start: nat, from: Array<T>, fromStart: nat, fromEnd: nat)
+    method WriteRange(start: nat, from: seq<T>)
+      requires Valid()
+      requires start <= Length()
+      requires start + |from| <= Length()
+      modifies Repr
+      ensures Valid()
+      ensures Repr == old(Repr)
+      ensures values == 
+        old(values)[..start] + 
+        seq(|from|, i requires 0 <= i < |from| => Set(from[i])) + 
+        old(values)[(start + |from|)..]
+    {
+      forall i | 0 <= i < |from| {
+        valuesArray[start + i] := Set(from[i]);
+      }
+      values := valuesArray[..];
+    }
+
+    method WriteRangeArray(start: nat, from: Array<T>, fromStart: nat, fromEnd: nat)
       requires Valid()
       requires from.Valid()
-      requires start < Length()
+      requires start <= Length()
       requires fromStart <= fromEnd <= from.Length()
       requires start + (fromEnd - fromStart) <= Length()
       requires forall i | fromStart <= i < fromEnd :: from.values[i].Set?
       requires Repr !! from.Repr
       modifies Repr
+      ensures Valid()
+      ensures Repr == old(Repr)
       ensures values == 
         old(values)[..start] + 
         from.values[fromStart..fromEnd] + 
         old(values)[(start + (fromEnd - fromStart))..]
-      {
-        var n := fromEnd - fromStart;
-        forall i | 0 <= i < n {
-          valuesArray[start + i] := Set(from.Read(fromStart + i));
-        }
-        values := valuesArray[..];
+    {
+      var n := fromEnd - fromStart;
+      forall i | 0 <= i < n {
+        valuesArray[start + i] := Set(from.Read(fromStart + i));
       }
+      values := valuesArray[..];
+    }
   }
 }
